Cslib/Computability/Machines/MultiTapeTuring/Routines/ListIteration.lean
@@ -26,29 +26,19 @@ public def run_list {k : ℕ} (i : Fin k) (tm : MultiTapeTM k Char) :
 
 /-- If `tm` computes a function `f` that acts like a folding function, the result of using
 `run_list` is a fold with accumulator on tape `j`. -/
-public lemma run_list_fold {k : ℕ} (i j : Fin k) (h_neq : i ≠ j) {tm : MultiTapeTM k Char}
-  (f : Data → TapeView → TapeView)
-  (h_comp : computes_function_read_update tm f i j h_neq)
-  (views : Fin k → TapeView) :
-  (run_list i tm).eval_struct views = some (Function.update views j
-      (((views i).currentList?.map
-        (fun ls => ls.foldl (fun acc d => f d acc) (views j))).getD (views j))) := by
+@[simp, grind =>]
+public lemma run_list_fold {k : ℕ} (i j : Fin k) (h_neq : i ≠ j)
+  {α : Type} [StrEnc α]
+  {tm : MultiTapeTM k Char}
+  (f : α → TapeView → TapeView)
+  (h_comp : computes_function_read_update tm f i j h_neq) :
+  computes_function_read_update (α := List α) (run_list i tm)
+    (fun ls => ls.foldl (fun acc d => f d acc)) i j h_neq := by
   sorry
 
 public def any_list {k : ℕ}
     (tm : MultiTapeTM k Char) (i j : Fin k) (_h_neq : i ≠ j) : MultiTapeTM k Char :=
   pushList (StrEnc.toData false) j ;ₜ run_list i (tm ;ₜ combineOrUpdate j)
-
-public theorem any_list_eval_struct {k : ℕ} (i j : Fin k)
-    (h_neq : i ≠ j)
-    {tm : MultiTapeTM k Char}
-    {f : Data → Bool}
-    (h_comp : computes_function_read_push tm f i j h_neq)
-    (views : Fin k → TapeView) :
-    (any_list tm i j h_neq).eval_struct views = some (Function.update views j
-      (((views i).currentList?.map
-        fun ls => (views j).pushList (StrEnc.toData (ls.any f))).getD (views j))) := by
-  sorry
 
 @[simp, grind =>]
 public theorem any_list.computes_fun {k : ℕ} {i j : Fin k}
